counterexample old attempt

theories/Logic/inverse_omega_neg.v
@@ -11,6 +11,7 @@ From Systems Require Import PA_omega.
 From Systems Require Import proof_trees.
 From Systems Require Import substitute.
 Require Import Lia.
+Require Import List.
 
 Definition associativity_1' (P : ptree) : ptree :=
 match ptree_formula P, ptree_deg P, ptree_ord P with
@@ -91,6 +92,32 @@ intros. induction A.
 - unfold within_f. unfold contains_f in H. case (eq_f (univ n A) B) eqn:X. inversion H. auto.
 Qed. 
 
+Lemma not_contain_no_change : forall A B C S, contains_f A B = false -> formula_sub_ind A B C S = A.
+Proof.
+intros A. induction A; intros.
+- case (subst_ind_fit (atom a) S) eqn:Y. rewrite sub_fit_true; auto. unfold formula_sub_ind_fit. unfold contains_f in H. case (eq_f (atom a) B) eqn:X. inversion H. auto.
+  rewrite sub_fit_false; auto.
+- case (subst_ind_fit (neg A) S) eqn:Y. rewrite sub_fit_true; auto. unfold formula_sub_ind_fit. unfold contains_f in H. case (eq_f (neg A) B) eqn:X. inversion H. auto.
+  rewrite sub_fit_false; auto.
+- case (subst_ind_fit (lor A1 A2) S) eqn:Y. rewrite sub_fit_true; auto. unfold formula_sub_ind_fit. fold formula_sub_ind_fit. destruct S; inversion Y. apply and_bool_prop in H1. destruct H1 as [Z1 Z2]. unfold contains_f in H. fold contains_f in H. case (eq_f (lor A1 A2) B) eqn:X. inversion H. case (contains_f A1 B) eqn:X1. inversion H. case (contains_f A2 B) eqn:X2. inversion H. rewrite <- sub_fit_true; auto. rewrite <- sub_fit_true; auto. rewrite IHA1; auto. rewrite IHA2; auto. 
+  rewrite sub_fit_false; auto.
+- case (subst_ind_fit (univ n A) S) eqn:Y. rewrite sub_fit_true; auto. unfold formula_sub_ind_fit. unfold contains_f in H. case (eq_f (univ n A) B) eqn:X. inversion H. auto.
+  rewrite sub_fit_false; auto.
+Qed. 
+
+Lemma not_contain_no_change_fit : forall A B C S, contains_f A B = false -> formula_sub_ind_fit A B C S = A.
+Proof.
+intros A. induction A; intros.
+- case (subst_ind_fit (atom a) S) eqn:Y; unfold formula_sub_ind_fit. unfold contains_f in H. case (eq_f (atom a) B) eqn:X. inversion H. auto.
+  destruct S; inversion Y; auto.  case (eq_f (atom a) B) eqn:X; auto.
+- case (subst_ind_fit (neg A) S) eqn:Y; unfold formula_sub_ind_fit. unfold contains_f in H. case (eq_f (neg A) B) eqn:X. inversion H. auto.
+  destruct S; inversion Y; auto.  case (eq_f (neg A) B) eqn:X; auto.
+- case (subst_ind_fit (lor A1 A2) S) eqn:Y; unfold formula_sub_ind_fit; fold formula_sub_ind_fit. destruct S; inversion Y. apply and_bool_prop in H1. destruct H1 as [Z1 Z2]. unfold contains_f in H. fold contains_f in H. case (eq_f (lor A1 A2) B) eqn:X. inversion H. case (contains_f A1 B) eqn:X1. inversion H. case (contains_f A2 B) eqn:X2. inversion H. rewrite IHA1; auto. rewrite IHA2; auto. 
+  destruct S; inversion Y; auto. unfold contains_f in H. fold contains_f in H. case (eq_f (lor A1 A2) B) eqn:X. inversion H. case (contains_f A1 B) eqn:X1. inversion H. case (contains_f A2 B) eqn:X2. inversion H. rewrite IHA1; auto. rewrite IHA2; auto. 
+- case (subst_ind_fit (univ n A) S) eqn:Y; unfold formula_sub_ind_fit. unfold contains_f in H. case (eq_f (univ n A) B) eqn:X. inversion H. auto.
+  destruct S; inversion Y; auto.  case (eq_f (univ n A) B) eqn:X; auto.
+Qed. 
+
 Lemma contains_symm : forall A B C, eq_f (lor A B) C = false -> contains_f (lor A B) C = true -> contains_f (lor B A) C = true.
 Proof. 
 intros. unfold contains_f in *. fold contains_f in *. rewrite H in H0. apply or_bool_prop in H0. destruct H0; rewrite H0; case (eq_f (lor B A) C); auto. case (contains_f B C); auto.
@@ -138,57 +165,344 @@ intros A. induction A.
 - intros. unfold contains_f in H0. case (eq_f (univ n A) B) eqn:Y. apply f_eq_decid in Y. destruct Y. auto. inversion H0.
 Qed.
 
+Fixpoint univ_counter_example 
+  (P : ptree) (E : formula) (n : nat) (S : subst_ind) : list term :=
+match P, S with
+| deg_up d P', _ => univ_counter_example P' E n S
+
+| ord_up alpha P', _ => univ_counter_example P' E n S
+
+| node A, _ => nil
+
+| exchange_ab A B d alpha P', lor_ind S_A S_B => univ_counter_example P' E n (lor_ind S_B S_A)
+
+| exchange_cab C A B d alpha P', lor_ind (lor_ind S_C S_B) S_A  => univ_counter_example P' E n (lor_ind (lor_ind S_C S_A) S_B)
+
+| exchange_abd A B D d alpha P', lor_ind (lor_ind S_B S_A) S_D => univ_counter_example P' E n (lor_ind (lor_ind S_A S_B) S_D)
+
+| exchange_cabd C0 A B D d alpha P', lor_ind (lor_ind (lor_ind S_C S_B) S_A) S_D => univ_counter_example P' E n (lor_ind (lor_ind (lor_ind S_C S_A) S_B) S_D)
+
+| contraction_a A d alpha P', _ => univ_counter_example P' E n (lor_ind S S)
+
+| contraction_ad A D d alpha P', lor_ind S_A S_D => univ_counter_example P' E n (lor_ind (lor_ind S_A S_A) S_D)
+
+| weakening_ad A D d alpha P', lor_ind S_A S_D => match contains_f A (neg (univ n E)) with
+    | true => (cons zero (univ_counter_example P' E n S_D))
+    | false => (univ_counter_example P' E n S_D)
+    end
+
+| demorgan_ab A B d1 d2 alpha1 alpha2 P1 P2, _ => nil
+
+| demorgan_abd A B D d1 d2 alpha1 alpha2 P1 P2, lor_ind S_AB S_D => (univ_counter_example P1 E n (lor_ind (0) S_D)) ++ (univ_counter_example P2 E n (lor_ind (0) S_D))
+
+| negation_a A d alpha P', _ => nil
+
+| negation_ad A D d alpha P', lor_ind S_A S_D => (univ_counter_example P' E n (lor_ind S_A S_D))
+
+| quantification_a A k t d alpha P', _ =>
+    (match eq_f A E, eq_nat k n, S with
+          | true, true, (1) => (cons t nil)
+          | _,_,_ => univ_counter_example P' E n S
+      end)
+
+| quantification_ad A D k t d alpha P', lor_ind S_A S_D =>
+    (match eq_f A E, eq_nat k n, S_A with
+    | true, true, (1) => (cons t (univ_counter_example P' E n (lor_ind (0) S_D)))
+    | _, _, _ => univ_counter_example P' E n S
+    end)
+
+| w_rule_a A k d alpha g, _ => nil
+
+| w_rule_ad A D k d alpha g, lor_ind S_A S_D => univ_counter_example (g 0) E n S_D
+
+| cut_ca C0 A d1 d2 alpha1 alpha2 P1 P2, _ => univ_counter_example P1 E n (lor_ind S (non_target A))
+
+| cut_ad A D d1 d2 alpha1 alpha2 P1 P2, _ => univ_counter_example P2 E n (lor_ind (0) S)
+
+| cut_cad C0 A D d1 d2 alpha1 alpha2 P1 P2, lor_ind S_C S_D => (univ_counter_example P1 E n (lor_ind S_C (non_target A))) ++ (univ_counter_example P2 E n (lor_ind (0) S_D))
+
+| _, _ => nil
+end.
+
+Lemma contains_has_counter : forall (P : ptree) (E : formula) (n : nat), contains_f (ptree_formula P) (neg (univ n E)) = true -> length (univ_counter_example P E n (within_f (ptree_formula P) (neg (univ n E)))) > 0.
+Proof.
+Admitted.
+
+Definition bad_head (L : list term) : term. destruct L. exact zero. exact t. Defined.
+
 Definition neg_invert (alpha : ord ) : Type := forall (P : ptree) (A B : formula) (n d : nat),
       contains_f A (neg (univ n B)) = true -> (P_proves P A d alpha ->
-            { t : term & provable (formula_sub_ind A (neg (univ n B)) (substitution (neg B) n t) (within_f A (neg (univ n B)))) d alpha}).
+            { t : term & provable (formula_sub_ind A (neg (univ n B)) (substitution (neg B) n t) (within_f A (neg (univ n B)))) d alpha & closed_t t = true}).
 
-Lemma w_rule_invertible_a : forall (P : ptree) (A B : formula) (n d : nat) (alpha : ord),
+Lemma w_rule_invertible_a : forall (P : ptree) (A B : formula) (n d : nat) (alpha : ord) (C : contains_f (ptree_formula P) (neg (univ n B)) = true), (P_proves P A d alpha ->
+      forall (S : subst_ind), subst_ind_fit A S = true -> 
+            provable (formula_sub_ind A (neg (univ n B)) (substitution (neg B) n (bad_head (univ_counter_example P B n (within_f (ptree_formula P) (neg (univ n B)))))) S) d alpha).
+Proof.
+unfold provable. induction P; intros A B m d alpha C [[[Ht1 Ht2] Ht3] Ht4] S HS.
+- destruct Ht2. simpl in Ht3. apply IHP; auto. repeat split; auto. lia.
+- destruct Ht2 as [[Ht2a Ht2b] Ht2c]. simpl in Ht1,Ht3,Ht4. destruct Ht4.
+  assert (P_proves P A (ptree_deg P) (ptree_ord P)). repeat split; auto. destruct (IHP A B m (ptree_deg P) (ptree_ord P) C X S HS) as [P1 [[[HP1 HP2] HP3] HP4]]. exists (ord_up o P1). destruct HP4. repeat split; simpl; auto. lia.
+- rewrite Ht1 in C. unfold contains_f in C. fold contains_f in C. destruct A; inversion C.
+  + admit.
+  + admit. (* simpl in Ht1. inversion Ht1. case (eq_f (neg A) (neg (univ m B))) eqn:X. inversion X. apply f_eq_decid in H1. rewrite H1 in *. simpl in Ht1. rewrite Ht1 in Ht2. inversion Ht2. inversion C. simpl in Ht1. rewrite Ht1 in Ht2. inversion Ht2. *)
+- simpl in Ht1,Ht3,Ht4. destruct Ht2 as [[[Ht2a Ht2b] Ht2c] Ht2d]. destruct Ht1,Ht4.
+  assert (P_proves P (lor f f0) (ptree_deg P) (ptree_ord P)). repeat split; auto. assert (eq_f (lor f0 f) (neg (univ m B)) = false) as X0. auto. destruct S; inversion HS. apply and_bool_prop in H0. destruct H0.
+  assert (subst_ind_fit (lor f f0) (lor_ind S2 S1) = true) as HS'. simpl. rewrite H,H0. auto. rewrite Ht2a in IHP.
+  destruct (IHP (lor f f0) B m (ptree_deg P) (ptree_ord P) (contains_symm _ _ _ X0 C) X _ HS') as [P1 [[[HP1 HP2] HP3] HP4]]. exists (exchange_ab (formula_sub_ind f (neg (univ m B)) (substitution (neg B) m (bad_head (univ_counter_example P B m (within_f (ptree_formula P) (neg (univ m B)))))) S2) (formula_sub_ind f0 (neg (univ m B)) (substitution (neg B) m (bad_head (univ_counter_example P B m (within_f (ptree_formula P) (neg (univ m B)))))) S1) (ptree_deg P1) o P1). destruct HP4. repeat split; simpl; auto.
+  rewrite and_bool_symm; auto. rewrite Ht2a. rewrite <- formula_sub_ind_lor; auto. simpl. rewrite H,H0. simpl. auto. rewrite HP1. rewrite Ht2a. rewrite formula_sub_ind_lor; auto. lia.
+- simpl in Ht1,Ht3,Ht4. destruct Ht2 as [[[Ht2a Ht2b] Ht2c] Ht2d]. destruct Ht1,Ht4.
+  assert (P_proves P (lor (lor f f0) f1) (ptree_deg P) (ptree_ord P)). repeat split; auto. assert (eq_f (lor (lor f f1) f0) (neg (univ m B)) = false) as X0. auto. assert (eq_f (lor f0 f) (neg (univ m B)) = false) as X1. auto. destruct S; inversion HS. destruct S1; inversion H0. clear H1. apply and_bool_prop in H0. destruct H0. apply and_bool_prop in H. destruct H.
+  assert (subst_ind_fit (lor (lor f f0) f1) (lor_ind (lor_ind S1_1 S2) S1_2) = true) as HS'. simpl. rewrite H,H0,H1. auto. rewrite Ht2a in *.
+  destruct (IHP (lor (lor f f0) f1) B m (ptree_deg P) (ptree_ord P) (contains_swap_end _ _ _ _ X0 X1 C) X _ HS') as [P1 [[[HP1 HP2] HP3] HP4]]. 
+  exists (exchange_cab (formula_sub_ind f (neg (univ m B)) (substitution (neg B) m (bad_head (univ_counter_example P B m (within_f (ptree_formula P) (neg (univ m B)))))) S1_1) (formula_sub_ind f0 (neg (univ m B)) (substitution (neg B) m (bad_head (univ_counter_example P B m (within_f (ptree_formula P) (neg (univ m B)))))) S2) (formula_sub_ind f1 (neg (univ m B)) (substitution (neg B) m (bad_head (univ_counter_example P B m (within_f (ptree_formula P) (neg (univ m B)))))) S1_2) (ptree_deg P1) o P1). destruct HP4. rewrite Ht2a. repeat split; simpl; auto.
+  rewrite H,H1,H0. simpl. repeat rewrite sub_fit_true; auto. repeat rewrite <- formula_sub_ind_lor; auto. rewrite H0,H. auto. lia.
+- simpl in Ht1,Ht3,Ht4. destruct Ht2 as [[[Ht2a Ht2b] Ht2c] Ht2d]. destruct Ht1,Ht4. rewrite Ht2a in *.
+  assert (P_proves P (lor (lor f f0) f1) (ptree_deg P) (ptree_ord P)). repeat split; auto. assert (eq_f (lor (lor f0 f) f1) (neg (univ m B)) = false) as X0. auto. assert (eq_f (lor f0 f) (neg (univ m B)) = false) as X1. auto. destruct S; inversion HS. destruct S1; inversion H0. clear H1. apply and_bool_prop in H0. destruct H0. apply and_bool_prop in H. destruct H.
+  assert (subst_ind_fit (lor (lor f f0) f1) (lor_ind (lor_ind S1_2 S1_1) S2) = true) as HS'; simpl; rewrite H,H1,H0; simpl; auto.
+  destruct (IHP (lor (lor f f0) f1) B m (ptree_deg P) (ptree_ord P) (contains_swap_start _ _ _ _ X0 X1 C) X _ HS') as [P1 [[[HP1 HP2] HP3] HP4]].
+  exists (exchange_abd (formula_sub_ind f (neg (univ m B)) (substitution (neg B) m (bad_head (univ_counter_example P B m (within_f (ptree_formula P) (neg (univ m B)))))) S1_2) (formula_sub_ind f0 (neg (univ m B)) (substitution (neg B) m (bad_head (univ_counter_example P B m (within_f (ptree_formula P) (neg (univ m B)))))) S1_1) (formula_sub_ind f1 (neg (univ m B)) (substitution (neg B) m (bad_head (univ_counter_example P B m (within_f (ptree_formula P) (neg (univ m B)))))) S2) (ptree_deg P1) o P1). destruct HP4. rewrite Ht2a. repeat split; simpl; auto.
+  repeat rewrite sub_fit_true; auto. repeat rewrite <- formula_sub_ind_lor; auto. rewrite H,H1. auto. lia.
+- simpl in Ht1,Ht3,Ht4. destruct Ht2 as [[[Ht2a Ht2b] Ht2c] Ht2d]. destruct Ht1,Ht4. rewrite Ht2a in *.
+  assert (P_proves P (lor (lor (lor f f0) f1) f2) (ptree_deg P) (ptree_ord P)). repeat split; auto. assert (eq_f (lor (lor (lor f f1) f0) f2) (neg (univ m B)) = false) as X0. auto. assert (eq_f (lor (lor f f1) f0) (neg (univ m B)) = false) as X1. auto. assert (eq_f (lor f f1) (neg (univ m B)) = false) as X2. auto. destruct S; inversion HS. destruct S1; inversion H0. clear H1. destruct S1_1; inversion H0. clear H1. apply and_bool_prop in H0. destruct H0. apply and_bool_prop in H. destruct H. apply and_bool_prop in H. destruct H.
+  assert (subst_ind_fit (lor (lor ( lor f f0) f1) f2) (lor_ind (lor_ind (lor_ind S1_1_1 S1_2) S1_1_2) S2) = true) as HS'; simpl; rewrite H,H1,H0,H2; simpl; auto.
+  destruct (IHP (lor (lor (lor f f0) f1) f2) B m (ptree_deg P) (ptree_ord P) (contains_swap_mid _ _ _ _ _ X0 X1 X2 C) X _ HS') as [P1 [[[HP1 HP2] HP3] HP4]].
+  exists (exchange_cabd (formula_sub_ind f (neg (univ m B)) (substitution (neg B) m (bad_head (univ_counter_example P B m (within_f (ptree_formula P) (neg (univ m B)))))) S1_1_1) (formula_sub_ind f0 (neg (univ m B)) (substitution (neg B) m (bad_head (univ_counter_example P B m (within_f (ptree_formula P) (neg (univ m B)))))) S1_2) (formula_sub_ind f1 (neg (univ m B)) (substitution (neg B) m (bad_head (univ_counter_example P B m (within_f (ptree_formula P) (neg (univ m B)))))) S1_1_2) (formula_sub_ind f2 (neg (univ m B)) (substitution (neg B) m (bad_head (univ_counter_example P B m (within_f (ptree_formula P) (neg (univ m B)))))) S2) (ptree_deg P1) o P1). destruct HP4. rewrite Ht2a. repeat split; simpl; auto.
+  repeat rewrite sub_fit_true; auto. repeat rewrite <- formula_sub_ind_lor; simpl; auto; try rewrite H; try rewrite H2; try rewrite H1; auto. lia.
+- simpl in Ht1,Ht3,Ht4. destruct Ht2 as [[[Ht2a Ht2b] Ht2c] Ht2d]. destruct Ht1,Ht4. rewrite Ht2a in *.
+  assert (P_proves P (lor f f) (ptree_deg P) (ptree_ord P)). repeat split; auto.
+  assert (subst_ind_fit (lor f f) (lor_ind S S) = true) as HS'; simpl; try rewrite HS; auto.
+  destruct (IHP (lor f f) B m (ptree_deg P) (ptree_ord P) (contains_weaken  _ f _ C) X _ HS') as [P1 [[[HP1 HP2] HP3] HP4]]. exists (contraction_a (formula_sub_ind f (neg (univ m B)) (substitution (neg B) m (bad_head (univ_counter_example P B m (within_f (ptree_formula P) (neg (univ m B)))))) S) (ptree_deg P1) o P1). destruct HP4. rewrite Ht2a. repeat split; simpl; auto.
+  rewrite <- formula_sub_ind_lor. auto. rewrite HS; auto. lia.
+- simpl in Ht1,Ht3,Ht4. destruct Ht2 as [[[Ht2a Ht2b] Ht2c] Ht2d]. destruct Ht1,Ht4. rewrite Ht2a in *.
+  assert (P_proves P (lor (lor f f) f0) (ptree_deg P) (ptree_ord P)). repeat split; auto. assert (eq_f (lor (lor f f0) f) (neg (univ m B)) = false) as X0. auto. assert (eq_f (lor f f0) (neg (univ m B)) = false) as X1. auto.
+  destruct S; inversion HS. apply and_bool_prop in H0. destruct H0. simpl. rewrite H,H0. simpl. assert (subst_ind_fit (lor (lor f f) f0) (lor_ind (lor_ind S1 S1) S2) = true) as HS'; simpl; try rewrite H; try rewrite H0; auto.
+  destruct (IHP (lor (lor f f) f0) B m (ptree_deg P) (ptree_ord P) (contains_swap_end _ _ _ _ X0 X1 (contains_weaken  _ f _ C)) X _ HS') as [P1 [[[HP1 HP2] HP3] HP4]]. exists (contraction_ad (formula_sub_ind f (neg (univ m B)) (substitution (neg B) m (bad_head (univ_counter_example P B m (within_f (ptree_formula P) (neg (univ m B)))))) S1) (formula_sub_ind f0 (neg (univ m B)) (substitution (neg B) m (bad_head (univ_counter_example P B m (within_f (ptree_formula P) (neg (univ m B)))))) S2) (ptree_deg P1) o P1). destruct HP4. rewrite Ht2a. repeat split; simpl; auto.
+  repeat rewrite sub_fit_true; auto. repeat rewrite <- formula_sub_ind_lor; auto. rewrite H. auto. lia.
+- simpl in Ht1,Ht3,Ht4. destruct Ht2 as [[[[Ht2a Ht2b] Ht2c] Ht2d] Ht2e]. rewrite Ht2a in *. destruct Ht1. simpl in C. apply or_bool_prop in C. destruct S; inversion HS. apply and_bool_prop in H0. destruct H0. case (contains_f f0 (neg (univ m B))) eqn:Y.
+  + assert (P_proves P f0 (ptree_deg P) (ptree_ord P)). repeat split; auto.
+    destruct (IHP f0 B m (ptree_deg P) (ptree_ord P) Y X _ H0) as [P1 [[[HP1 HP2] HP3] HP4]]. exists (weakening_ad (formula_sub_ind f (neg (univ m B)) (substitution (neg B) m (bad_head (univ_counter_example P B m (within_f (ptree_formula P) (neg (univ m B)))))) S1) (formula_sub_ind f0 (neg (univ m B)) (substitution (neg B) m (bad_head (univ_counter_example P B m (within_f (ptree_formula P) (neg (univ m B)))))) S2) (ptree_deg P1) o P1). destruct HP4. rewrite Ht2a. repeat split; simpl; auto.
+    rewrite H,H0. simpl. repeat rewrite sub_fit_true; auto. admit. apply formula_sub_ind_closed; auto. intros. apply closed_univ_sub; auto. admit. lia.
+  + exists (weakening_ad (formula_sub_ind f (neg (univ m B)) (substitution (neg B) m (represent 0)) S1) f0 n o P). repeat split; auto.
+    simpl. rewrite H,H0. simpl. repeat rewrite sub_fit_true; auto. rewrite (not_contain_no_change_fit _ _ _ _ Y); auto. destruct C. rewrite H1. simpl. auto. inversion H1. apply formula_sub_ind_closed; auto. intros. apply closed_univ_sub; auto.
+- admit.
+- admit.
+- simpl in Ht1,Ht3,Ht4. destruct Ht2 as [[[Ht2a Ht2b] Ht2c] Ht2d]. destruct Ht1,Ht4. simpl in C. inversion C.
+- simpl in Ht1,Ht3,Ht4. destruct Ht2 as [[[Ht2a Ht2b] Ht2c] Ht2d]. destruct Ht1,Ht4. simpl in C.  
+  assert (P_proves P (lor f f0) (ptree_deg P) (ptree_ord P)). repeat split; auto. assert (eq_f (lor f0 f) (neg (univ m B)) = false) as X0. auto.
+  destruct S; inversion HS. assert (subst_ind_fit f0 S2 = true). destruct S1; auto. inversion H0. rewrite Ht2a in *.
+  assert (subst_ind_fit (lor f f0) (lor_ind (non_target f) S2) = true) as HS'. simpl. rewrite non_target_fit. rewrite H. auto.
+  destruct (IHP (lor f f0) B m (ptree_deg P) (ptree_ord P) (contains_symm _ _ _ X0 (contains_weaken _ _ _ C)) X _ HS') as [P1 [[[HP1 HP2] HP3] HP4]].
+  exists (negation_ad f (formula_sub_ind f0 (neg (univ m B)) (substitution (neg B) m (bad_head (univ_counter_example P B m (within_f (ptree_formula P) (neg (univ m B)))))) S2) (ptree_deg P1) o P1). destruct HP4. repeat split; simpl; auto.
+  rewrite H0. rewrite Ht2a. repeat rewrite sub_fit_true; auto. simpl.  admit. rewrite HP1. rewrite Ht2a. simpl. rewrite non_target_fit. rewrite H. simpl. rewrite non_target_sub'. rewrite sub_fit_true; auto. lia.
+- simpl in Ht1,Ht3,Ht4. destruct Ht2 as [[[[Ht2a Ht2b] Ht2c] Ht2d] Ht2e]. destruct Ht1,Ht4. simpl in C. case (eq_nat n m) eqn:Y; inversion C. case (eq_f f B) eqn:Y1; inversion C. apply nat_eq_decid in Y. destruct Y. apply f_eq_decid in Y1. destruct Y1. destruct S; inversion HS.
+  + simpl. rewrite eq_nat_refl. rewrite eq_f_refl. simpl. exists (quantification_a f n t n0 o P). repeat split; auto.
+  + exists (ord_up (ord_succ o) P). simpl. rewrite eq_nat_refl. rewrite eq_f_refl. simpl. repeat split; simpl; auto; try rewrite Ht2e. apply ord_succ_monot. apply ord_succ_nf. apply ptree_ord_nf. auto. lia. 
+- simpl in Ht1,Ht3,Ht4. destruct Ht2 as [[[[Ht2a Ht2b] Ht2c] Ht2d] Ht2e]. destruct Ht1,Ht4. simpl in C. destruct S; inversion HS. destruct S1; inversion H0; clear H0; rewrite Ht2a in *.
+  + simpl. rewrite H1. case (eq_nat n m) eqn:Y; case (eq_f f B) eqn:Y1; simpl.
+    * case (contains_f f0 (neg (univ n f))) eqn:Y2.
+      --  apply nat_eq_decid in Y. destruct Y. apply f_eq_decid in Y1. destruct Y1. simpl. assert (P_proves P (lor (neg (substitution f n t)) f0) (ptree_deg P) (ptree_ord P)). repeat split; auto. assert (eq_f (lor f0 (neg (substitution f n t))) (neg (univ n f)) = false) as X0. auto.
+          assert (subst_ind_fit (lor (neg(substitution f n t)) f0) (lor_ind (0) S2) = true) as HS'. simpl. rewrite H1. auto.
+          destruct (IHP (lor (neg (substitution f n t)) f0) f n (ptree_deg P) (ptree_ord P) (contains_symm _ _ _ X0 (contains_weaken _ _ _ Y2)) X _ HS') as [P1 [[[HP1 HP2] HP3] HP4]].
+          exists (quantification_ad f (formula_sub_ind f0 (neg (univ n f)) (substitution (neg f) n (bad_head (univ_counter_example P f n (within_f (ptree_formula P) (neg (univ n f)))))) S2) n t (ptree_deg P1) o P1). simpl. repeat split; simpl; auto; try rewrite Ht2e. rewrite Ht2a. rewrite sub_fit_true; auto. simpl. assert (eq_f (substitution f n t) (univ n f) = false). admit. rewrite H.  rewrite HP1. simpl. rewrite H1. case (eq_f (substitution f n t) (univ n f)); rewrite sub_fit_true; auto. rewrite HP4. auto. lia.
+      --  apply nat_eq_decid in Y. destruct Y. apply f_eq_decid in Y1. destruct Y1. exists t; auto. exists (quantification_ad f f0 n t n0 o P). rewrite not_contain_no_change_fit; auto. repeat split; auto.
+    * simpl in C. apply nat_eq_decid in Y. destruct Y. assert (P_proves P (lor (neg (substitution f n t)) f0) (ptree_deg P) (ptree_ord P)). repeat split; auto. assert (eq_f (lor f0 (neg (substitution f n t))) (neg (univ n B)) = false) as X0. auto.
+      assert (subst_ind_fit (lor (neg(substitution f n t)) f0) (lor_ind (0) S2) = true) as HS'. simpl. rewrite H1. auto.
+      destruct (IHP (lor (neg (substitution f n t)) f0) B n (ptree_deg P) (ptree_ord P) (contains_symm _ _ _ X0 (contains_weaken _ _ _ C)) X _ HS') as [p HC [P1 [[[HP1 HP2] HP3] HP4]]].
+      exists p; auto. exists (quantification_ad f (formula_sub_ind f0 (neg (univ n B)) (substitution (neg B) n p) S2) n t (ptree_deg P1) o P1). repeat split; simpl; auto; try rewrite Ht2e. rewrite sub_fit_true; auto. rewrite HP1. simpl. rewrite H1. case (eq_f (substitution f n t) (univ n B)); rewrite sub_fit_true; auto. rewrite HP4. auto. lia.
+    * simpl in C. apply f_eq_decid in Y1. destruct Y1. assert (P_proves P (lor (neg (substitution f n t)) f0) (ptree_deg P) (ptree_ord P)). repeat split; auto. assert (eq_f (lor f0 (neg (substitution f n t))) (neg (univ m f)) = false) as X0. auto.
+      assert (subst_ind_fit (lor (neg(substitution f n t)) f0) (lor_ind (0) S2) = true) as HS'. simpl. rewrite H1. auto.
+      destruct (IHP (lor (neg (substitution f n t)) f0) f m (ptree_deg P) (ptree_ord P) (contains_symm _ _ _ X0 (contains_weaken _ _ _ C)) X _ HS') as [p HC [P1 [[[HP1 HP2] HP3] HP4]]].
+      exists p; auto. exists (quantification_ad f (formula_sub_ind f0 (neg (univ m f)) (substitution (neg f) m p) S2) n t (ptree_deg P1) o P1). repeat split; simpl; auto; try rewrite Ht2e. rewrite sub_fit_true; auto. rewrite HP1. simpl. rewrite H1. case (eq_f (substitution f n t) (univ m f)); rewrite sub_fit_true; auto. rewrite HP4. auto. lia.
+    * simpl in C. assert (P_proves P (lor (neg (substitution f n t)) f0) (ptree_deg P) (ptree_ord P)). repeat split; auto. assert (eq_f (lor f0 (neg (substitution f n t))) (neg (univ m B)) = false) as X0. auto.
+      assert (subst_ind_fit (lor (neg(substitution f n t)) f0) (lor_ind (0) S2) = true) as HS'. simpl. rewrite H1. auto.
+      destruct (IHP (lor (neg (substitution f n t)) f0) B m (ptree_deg P) (ptree_ord P) (contains_symm _ _ _ X0 (contains_weaken _ _ _ C)) X _ HS') as [p HC [P1 [[[HP1 HP2] HP3] HP4]]].
+      exists p; auto. exists (quantification_ad f (formula_sub_ind f0 (neg (univ m B)) (substitution (neg B) m p) S2) n t (ptree_deg P1) o P1). repeat split; simpl; auto; try rewrite Ht2e. rewrite sub_fit_true; auto. rewrite HP1. simpl. rewrite H1. case (eq_f (substitution f n t) (univ m B)); rewrite sub_fit_true; auto. rewrite HP4. auto. lia.
+    + simpl. rewrite H1. case (eq_nat n m) eqn:Y; case (eq_f f B) eqn:Y1; simpl.
+      * case (contains_f f0 (neg (univ n f))) eqn:Y2.
+        --  apply nat_eq_decid in Y. destruct Y. apply f_eq_decid in Y1. destruct Y1. simpl. assert (P_proves P (lor (neg (substitution f n t)) f0) (ptree_deg P) (ptree_ord P)). repeat split; auto. assert (eq_f (lor f0 (neg (substitution f n t))) (neg (univ n f)) = false) as X0. auto.
+            assert (subst_ind_fit (lor (neg(substitution f n t)) f0) (lor_ind (1) S2) = true) as HS'. simpl. rewrite H1. auto.
+            destruct (IHP (lor (neg (substitution f n t)) f0) f n (ptree_deg P) (ptree_ord P) (contains_symm _ _ _ X0 (contains_weaken _ _ _ Y2)) X _ HS') as [p HC [P1 [[[HP1 HP2] HP3] HP4]]].
+            exists p; auto. exists (ord_up (ord_succ o) P1). repeat split; simpl; auto; try rewrite Ht2e. rewrite HP1. simpl. rewrite H1. assert (eq_f (substitution f n t) (univ n f) = false). admit. rewrite H. admit. rewrite HP4. apply ord_succ_monot. apply ord_succ_nf. apply ptree_ord_nf. auto. lia.
+        --  apply nat_eq_decid in Y. destruct Y. apply f_eq_decid in Y1. destruct Y1. exists t; auto. exists (ord_up (ord_succ (ptree_ord P)) P). rewrite not_contain_no_change_fit; auto. repeat split; simpl; auto. apply ord_succ_monot. apply ord_succ_nf. apply ptree_ord_nf. auto. lia. rewrite Ht2e. auto.
+      * simpl in C. apply nat_eq_decid in Y. destruct Y. assert (P_proves P (lor (neg (substitution f n t)) f0) (ptree_deg P) (ptree_ord P)). repeat split; auto. assert (eq_f (lor f0 (neg (substitution f n t))) (neg (univ n B)) = false) as X0. auto.
+        assert (subst_ind_fit (lor (neg(substitution f n t)) f0) (lor_ind (0) S2) = true) as HS'. simpl. rewrite H1. auto.
+        destruct (IHP (lor (neg (substitution f n t)) f0) B n (ptree_deg P) (ptree_ord P) (contains_symm _ _ _ X0 (contains_weaken _ _ _ C)) X _ HS') as [p HC [P1 [[[HP1 HP2] HP3] HP4]]].
+        exists p; auto. exists (quantification_ad f (formula_sub_ind f0 (neg (univ n B)) (substitution (neg B) n p) S2) n t (ptree_deg P1) o P1). repeat split; simpl; auto; try rewrite Ht2e. rewrite sub_fit_true; auto. rewrite HP1. simpl. rewrite H1. case (eq_f (substitution f n t) (univ n B)); rewrite sub_fit_true; auto. rewrite HP4. auto. lia.
+      * simpl in C. apply f_eq_decid in Y1. destruct Y1. assert (P_proves P (lor (neg (substitution f n t)) f0) (ptree_deg P) (ptree_ord P)). repeat split; auto. assert (eq_f (lor f0 (neg (substitution f n t))) (neg (univ m f)) = false) as X0. auto.
+        assert (subst_ind_fit (lor (neg(substitution f n t)) f0) (lor_ind (0) S2) = true) as HS'. simpl. rewrite H1. auto.
+        destruct (IHP (lor (neg (substitution f n t)) f0) f m (ptree_deg P) (ptree_ord P) (contains_symm _ _ _ X0 (contains_weaken _ _ _ C)) X _ HS') as [p HC [P1 [[[HP1 HP2] HP3] HP4]]].
+        exists p; auto. exists (quantification_ad f (formula_sub_ind f0 (neg (univ m f)) (substitution (neg f) m p) S2) n t (ptree_deg P1) o P1). repeat split; simpl; auto; try rewrite Ht2e. rewrite sub_fit_true; auto. rewrite HP1. simpl. rewrite H1. case (eq_f (substitution f n t) (univ m f)); rewrite sub_fit_true; auto. rewrite HP4. auto. lia.
+      * simpl in C. assert (P_proves P (lor (neg (substitution f n t)) f0) (ptree_deg P) (ptree_ord P)). repeat split; auto. assert (eq_f (lor f0 (neg (substitution f n t))) (neg (univ m B)) = false) as X0. auto.
+        assert (subst_ind_fit (lor (neg(substitution f n t)) f0) (lor_ind (0) S2) = true) as HS'. simpl. rewrite H1. auto.
+        destruct (IHP (lor (neg (substitution f n t)) f0) B m (ptree_deg P) (ptree_ord P) (contains_symm _ _ _ X0 (contains_weaken _ _ _ C)) X _ HS') as [p HC [P1 [[[HP1 HP2] HP3] HP4]]].
+        exists p; auto. exists (quantification_ad f (formula_sub_ind f0 (neg (univ m B)) (substitution (neg B) m p) S2) n t (ptree_deg P1) o P1). repeat split; simpl; auto; try rewrite Ht2e. rewrite sub_fit_true; auto. rewrite HP1. simpl. rewrite H1. case (eq_f (substitution f n t) (univ m B)); rewrite sub_fit_true; auto. rewrite HP4. auto. lia.
+- simpl in Ht1,Ht3,Ht4. destruct Ht1,Ht4. inversion C.
+- simpl in Ht1,Ht3,Ht4. destruct Ht1,Ht4. inversion C. simpl in Ht2. admit.
+- simpl in Ht1,Ht3,Ht4. destruct Ht2 as [[[[[[[Ht2a Ht2b] Ht2c] Ht2d] Ht2e] Ht2f] Ht2g] Ht2h]. destruct Ht1,Ht4.
+  assert (P_proves P1 (lor f f0) (ptree_deg P1) (ptree_ord P1)). repeat split; auto. assert (P_proves P2 (neg f0) (ptree_deg P2) (ptree_ord P2)). repeat split; auto. admit.
+- admit.
+- admit.
+Admitted.
+(*
+
+Lemma w_rule_invertible_a_shuffle : forall (B : formula) (n : nat), {t : term & closed_t t = true & forall (P : ptree) (A : formula) (d : nat) (alpha : ord),
+      contains_f A (neg (univ n B)) = true -> (P_proves P A d alpha -> forall (S : subst_ind), subst_ind_fit A S = true -> provable (formula_sub_ind A (neg (univ n B)) (substitution (neg B) n t) S) d alpha)}.
+Proof.
+unfold provable. intros. induction B.
+exists zero. auto. intros P.
+
+induction P; intros A d alpha C [[[Ht1 Ht2] Ht3] Ht4] S HS.
+- destruct Ht2. simpl in Ht3. apply IHP; repeat split; auto. lia.
+- destruct Ht2 as [[Ht2a Ht2b] Ht2c]. simpl in Ht1,Ht3,Ht4. destruct Ht4.
+  assert (P_proves P A (ptree_deg P) (ptree_ord P)). repeat split; auto. destruct (IHP A (ptree_deg P) (ptree_ord P) C X S HS) as [P1 [[[HP1 HP2] HP3] HP4]]. exists (ord_up o P1). destruct HP4. repeat split; simpl; auto. lia.
+- unfold contains_f in C. destruct A; inversion C. case (eq_f (neg A) (neg (univ n (atom a)))) eqn:X. inversion X. apply f_eq_decid in H1. rewrite H1 in *. simpl in Ht1. rewrite Ht1 in Ht2. inversion Ht2. inversion C. simpl in Ht1. rewrite Ht1 in Ht2. inversion Ht2.
+- simpl in Ht1,Ht3,Ht4. destruct Ht2 as [[[Ht2a Ht2b] Ht2c] Ht2d]. destruct Ht1,Ht4.
+  assert (P_proves P (lor f f0) (ptree_deg P) (ptree_ord P)). repeat split; auto. assert (eq_f (lor f0 f) (neg (univ n (atom a))) = false) as X0. auto. destruct S; inversion HS. apply and_bool_prop in H0. destruct H0.
+  assert (subst_ind_fit (lor f f0) (lor_ind S2 S1) = true) as HS'. simpl. rewrite H,H0. auto.
+  destruct (IHP (lor f f0) (ptree_deg P) (ptree_ord P) (contains_symm _ _ _ X0 C) X _ HS') as [P1 [[[HP1 HP2] HP3] HP4]]. exists (exchange_ab (formula_sub_ind f (neg (univ n (atom a))) (substitution (neg (atom a)) n zero) S2) (formula_sub_ind f0 (neg (univ n (atom a))) (substitution (neg (atom a)) n zero) S1) (ptree_deg P1) o P1). destruct HP4. repeat split; simpl; auto.
+  rewrite and_bool_symm; auto. repeat rewrite sub_fit_true; auto. rewrite <- formula_sub_ind_lor; auto. lia.
+- simpl in Ht1,Ht3,Ht4. destruct Ht2 as [[[Ht2a Ht2b] Ht2c] Ht2d]. destruct Ht1,Ht4.
+  assert (P_proves P (lor (lor f f0) f1) (ptree_deg P) (ptree_ord P)). repeat split; auto. assert (eq_f (lor (lor f f1) f0) (neg (univ n (atom a))) = false) as X0. auto. assert (eq_f (lor f0 f) (neg (univ n (atom a))) = false) as X1. auto. destruct S; inversion HS. destruct S1; inversion H0. clear H1. apply and_bool_prop in H0. destruct H0. apply and_bool_prop in H. destruct H.
+  assert (subst_ind_fit (lor (lor f f0) f1) (lor_ind (lor_ind S1_1 S2) S1_2) = true) as HS'. simpl. rewrite H,H0,H1. auto.
+  destruct (IHP (lor (lor f f0) f1) (ptree_deg P) (ptree_ord P) (contains_swap_end _ _ _ _ X0 X1 C) X _ HS') as [P1 [[[HP1 HP2] HP3] HP4]]. 
+  exists (exchange_cab (formula_sub_ind f (neg (univ n (atom a))) (substitution (neg (atom a)) n zero) S1_1) (formula_sub_ind f0 (neg (univ n (atom a))) (substitution (neg (atom a)) n zero) S2) (formula_sub_ind f1 (neg (univ n (atom a))) (substitution (neg (atom a)) n zero) S1_2) (ptree_deg P1) o P1). destruct HP4. repeat split; simpl; auto.
+  rewrite H,H1,H0. simpl. repeat rewrite sub_fit_true; auto. repeat rewrite <- formula_sub_ind_lor; auto. rewrite H0,H. auto. lia.
+- simpl in Ht1,Ht3,Ht4. destruct Ht2 as [[[Ht2a Ht2b] Ht2c] Ht2d]. destruct Ht1,Ht4.
+  assert (P_proves P (lor (lor f f0) f1) (ptree_deg P) (ptree_ord P)). repeat split; auto. assert (eq_f (lor (lor f0 f) f1) (neg (univ n (atom a))) = false) as X0. auto. assert (eq_f (lor f0 f) (neg (univ n (atom a))) = false) as X1. auto. destruct S; inversion HS. destruct S1; inversion H0. clear H1. apply and_bool_prop in H0. destruct H0. apply and_bool_prop in H. destruct H.
+  assert (subst_ind_fit (lor (lor f f0) f1) (lor_ind (lor_ind S1_2 S1_1) S2) = true) as HS'; simpl; rewrite H,H1,H0; simpl; auto.
+  destruct (IHP (lor (lor f f0) f1) (ptree_deg P) (ptree_ord P) (contains_swap_start _ _ _ _ X0 X1 C) X _ HS') as [P1 [[[HP1 HP2] HP3] HP4]].
+  exists (exchange_abd (formula_sub_ind f (neg (univ n (atom a))) (substitution (neg (atom a)) n zero) S1_2) (formula_sub_ind f0 (neg (univ n (atom a))) (substitution (neg (atom a)) n zero) S1_1) (formula_sub_ind f1 (neg (univ n (atom a))) (substitution (neg (atom a)) n zero) S2) (ptree_deg P1) o P1). destruct HP4. repeat split; simpl; auto.
+  repeat rewrite sub_fit_true; auto. repeat rewrite <- formula_sub_ind_lor; auto. rewrite H,H1. auto. lia.
+- simpl in Ht1,Ht3,Ht4. destruct Ht2 as [[[Ht2a Ht2b] Ht2c] Ht2d]. destruct Ht1,Ht4.
+  assert (P_proves P (lor (lor (lor f f0) f1) f2) (ptree_deg P) (ptree_ord P)). repeat split; auto. assert (eq_f (lor (lor (lor f f1) f0) f2) (neg (univ n (atom a))) = false) as X0. auto. assert (eq_f (lor (lor f f1) f0) (neg (univ n (atom a))) = false) as X1. auto. assert (eq_f (lor f f1) (neg (univ n (atom a))) = false) as X2. auto. destruct S; inversion HS. destruct S1; inversion H0. clear H1. destruct S1_1; inversion H0. clear H1. apply and_bool_prop in H0. destruct H0. apply and_bool_prop in H. destruct H. apply and_bool_prop in H. destruct H.
+  assert (subst_ind_fit (lor (lor ( lor f f0) f1) f2) (lor_ind (lor_ind (lor_ind S1_1_1 S1_2) S1_1_2) S2) = true) as HS'; simpl; rewrite H,H1,H0,H2; simpl; auto.
+  destruct (IHP (lor (lor (lor f f0) f1) f2) (ptree_deg P) (ptree_ord P) (contains_swap_mid _ _ _ _ _ X0 X1 X2 C) X _ HS') as [P1 [[[HP1 HP2] HP3] HP4]].
+  exists (exchange_cabd (formula_sub_ind f (neg (univ n (atom a))) (substitution (neg (atom a)) n zero) S1_1_1) (formula_sub_ind f0 (neg (univ n (atom a))) (substitution (neg (atom a)) n zero) S1_2) (formula_sub_ind f1 (neg (univ n (atom a))) (substitution (neg (atom a)) n zero) S1_1_2) (formula_sub_ind f2 (neg (univ n (atom a))) (substitution (neg (atom a)) n zero) S2) (ptree_deg P1) o P1). destruct HP4. repeat split; simpl; auto.
+  repeat rewrite sub_fit_true; auto. repeat rewrite <- formula_sub_ind_lor; simpl; auto; try rewrite H; try rewrite H2; try rewrite H1; auto. lia.
+- simpl in Ht1,Ht3,Ht4. destruct Ht2 as [[[Ht2a Ht2b] Ht2c] Ht2d]. destruct Ht1,Ht4.
+  assert (P_proves P (lor f f) (ptree_deg P) (ptree_ord P)). repeat split; auto.
+  assert (subst_ind_fit (lor f f) (lor_ind S S) = true) as HS'; simpl; try rewrite HS; auto.
+  destruct (IHP (lor f f) (ptree_deg P) (ptree_ord P) (contains_weaken  _ f _ C) X _ HS') as [P1 [[[HP1 HP2] HP3] HP4]]. exists (contraction_a (formula_sub_ind f (neg (univ n (atom a))) (substitution (neg (atom a)) n zero) S) (ptree_deg P1) o P1). destruct HP4. repeat split; simpl; auto.
+  rewrite <- formula_sub_ind_lor. auto. rewrite HS; auto. lia.
+- simpl in Ht1,Ht3,Ht4. destruct Ht2 as [[[Ht2a Ht2b] Ht2c] Ht2d]. destruct Ht1,Ht4.
+  assert (P_proves P (lor (lor f f) f0) (ptree_deg P) (ptree_ord P)). repeat split; auto. assert (eq_f (lor (lor f f0) f) (neg (univ n (atom a))) = false) as X0. auto. assert (eq_f (lor f f0) (neg (univ n (atom a))) = false) as X1. auto.
+  destruct S; inversion HS. apply and_bool_prop in H0. destruct H0. simpl. rewrite H,H0. simpl. assert (subst_ind_fit (lor (lor f f) f0) (lor_ind (lor_ind S1 S1) S2) = true) as HS'; simpl; try rewrite H; try rewrite H0; auto.
+  destruct (IHP (lor (lor f f) f0) (ptree_deg P) (ptree_ord P) (contains_swap_end _ _ _ _ X0 X1 (contains_weaken  _ f _ C)) X _ HS') as [P1 [[[HP1 HP2] HP3] HP4]]. exists (contraction_ad (formula_sub_ind f (neg (univ n (atom a))) (substitution (neg (atom a)) n zero) S1) (formula_sub_ind f0 (neg (univ n (atom a))) (substitution (neg (atom a)) n zero) S2) (ptree_deg P1) o P1). destruct HP4. repeat split; simpl; auto.
+  repeat rewrite sub_fit_true; auto. repeat rewrite <- formula_sub_ind_lor; auto. rewrite H. auto. lia.
+- simpl in Ht1,Ht3,Ht4. destruct Ht2 as [[[[Ht2a Ht2b] Ht2c] Ht2d] Ht2e]. destruct Ht1. simpl in C. apply or_bool_prop in C. destruct S; inversion HS. apply and_bool_prop in H0. destruct H0. case (contains_f f0 (neg (univ n (atom a)))) eqn:Y.
+  + assert (P_proves P f0 (ptree_deg P) (ptree_ord P)). repeat split; auto.
+    destruct (IHP f0 (ptree_deg P) (ptree_ord P) Y X _ H0) as [P1 [[[HP1 HP2] HP3] HP4]]. exists (weakening_ad (formula_sub_ind f (neg (univ n (atom a))) (substitution (neg (atom a)) n zero) S1) (formula_sub_ind f0 (neg (univ n (atom a))) (substitution (neg (atom a)) n zero) S2) (ptree_deg P1) o P1). destruct HP4. repeat split; auto.
+    simpl. rewrite H,H0. simpl. repeat rewrite sub_fit_true; auto. apply formula_sub_ind_closed; auto. intros. rewrite closed_univ_sub; auto. simpl. lia.
+  + exists (weakening_ad (formula_sub_ind f (neg (univ n (atom a))) (substitution (neg (atom a)) n zero) S1) f0 n0 o P). repeat split; auto.
+    simpl. rewrite H,H0. simpl. repeat rewrite sub_fit_true; auto. rewrite (not_contain_no_change_fit _ _ _ _ Y); auto. apply formula_sub_ind_closed; auto. intros. apply closed_univ_sub; auto.
+- admit.
+- admit.
+- simpl in Ht1,Ht3,Ht4. destruct Ht2 as [[[Ht2a Ht2b] Ht2c] Ht2d]. destruct Ht1,Ht4. simpl in C. inversion C.
+- simpl in Ht1,Ht3,Ht4. destruct Ht2 as [[[Ht2a Ht2b] Ht2c] Ht2d]. destruct Ht1,Ht4. simpl in C.  
+  assert (P_proves P (lor f f0) (ptree_deg P) (ptree_ord P)). repeat split; auto. assert (eq_f (lor f0 f) (neg (univ n (atom a))) = false) as X0. auto.
+  destruct S; inversion HS. assert (subst_ind_fit f0 S2 = true). destruct S1; auto. inversion H0.
+  assert (subst_ind_fit (lor f f0) (lor_ind (non_target f) S2) = true) as HS'. simpl. rewrite non_target_fit. rewrite H. auto.
+  destruct (IHP (lor f f0) (ptree_deg P) (ptree_ord P) (contains_symm _ _ _ X0 (contains_weaken _ _ _ C)) X _ HS') as [P1 [[[HP1 HP2] HP3] HP4]].
+  exists (negation_ad f (formula_sub_ind f0 (neg (univ n (atom a))) (substitution (neg (atom a)) n zero) S2) (ptree_deg P1) o P1). destruct HP4. repeat split; simpl; auto.
+  rewrite H0. repeat rewrite sub_fit_true; auto. rewrite HP1. simpl. rewrite non_target_fit. rewrite H. simpl. rewrite non_target_sub'. rewrite sub_fit_true; auto. lia.
+- simpl in Ht1,Ht3,Ht4. destruct Ht2 as [[[[Ht2a Ht2b] Ht2c] Ht2d] Ht2e]. destruct Ht1,Ht4. simpl in C. case (eq_nat n n0) eqn:Y; inversion C. case (eq_f f (atom a)) eqn:Y1; inversion C. apply nat_eq_decid in Y. destruct Y. apply f_eq_decid in Y1. destruct Y1. destruct S; inversion HS.
+  + simpl. rewrite eq_nat_refl. rewrite eq_f_refl. simpl. exists (quantification_a f n t n1 o P). repeat split; auto.
+  + exists (ord_up (ord_succ o) P). simpl. rewrite eq_nat_refl. rewrite eq_f_refl. simpl. repeat split; simpl; auto; try rewrite Ht2e. apply ord_succ_monot. apply ord_succ_nf. apply ptree_ord_nf. auto. lia. 
+- simpl in Ht1,Ht3,Ht4. destruct Ht2 as [[[[Ht2a Ht2b] Ht2c] Ht2d] Ht2e]. destruct Ht1,Ht4. simpl in C. destruct S; inversion HS; rewrite H0. destruct S1; inversion H0; rewrite H1; clear H0.
+  + simpl. rewrite H1. case (eq_nat n m) eqn:Y; case (eq_f f B) eqn:Y1; simpl.
+    * case (contains_f f0 (neg (univ n f))) eqn:Y2.
+      --  apply nat_eq_decid in Y. destruct Y. apply f_eq_decid in Y1. destruct Y1. simpl. assert (P_proves P (lor (neg (substitution f n t)) f0) (ptree_deg P) (ptree_ord P)). repeat split; auto. assert (eq_f (lor f0 (neg (substitution f n t))) (neg (univ n f)) = false) as X0. auto.
+          assert (subst_ind_fit (lor (neg(substitution f n t)) f0) (lor_ind (0) S2) = true) as HS'. simpl. rewrite H1. auto.
+          destruct (IHP (lor (neg (substitution f n t)) f0) f n (ptree_deg P) (ptree_ord P) (contains_symm _ _ _ X0 (contains_weaken _ _ _ Y2)) X _ HS') as [p HC [P1 [[[HP1 HP2] HP3] HP4]]].
+          exists p; auto. exists (quantification_ad f (formula_sub_ind f0 (neg (univ n f)) (substitution (neg f) n p) S2) n t (ptree_deg P1) o P1). simpl. repeat split; simpl; auto; try rewrite Ht2e. rewrite sub_fit_true; auto. rewrite HP1. simpl. rewrite H1. case (eq_f (substitution f n t) (univ n f)); rewrite sub_fit_true; auto. rewrite HP4. auto. lia.
+      --  apply nat_eq_decid in Y. destruct Y. apply f_eq_decid in Y1. destruct Y1. exists t; auto. exists (quantification_ad f f0 n t n0 o P). rewrite not_contain_no_change_fit; auto. repeat split; auto.
+    * simpl in C. apply nat_eq_decid in Y. destruct Y. assert (P_proves P (lor (neg (substitution f n t)) f0) (ptree_deg P) (ptree_ord P)). repeat split; auto. assert (eq_f (lor f0 (neg (substitution f n t))) (neg (univ n B)) = false) as X0. auto.
+      assert (subst_ind_fit (lor (neg(substitution f n t)) f0) (lor_ind (0) S2) = true) as HS'. simpl. rewrite H1. auto.
+      destruct (IHP (lor (neg (substitution f n t)) f0) B n (ptree_deg P) (ptree_ord P) (contains_symm _ _ _ X0 (contains_weaken _ _ _ C)) X _ HS') as [p HC [P1 [[[HP1 HP2] HP3] HP4]]].
+      exists p; auto. exists (quantification_ad f (formula_sub_ind f0 (neg (univ n B)) (substitution (neg B) n p) S2) n t (ptree_deg P1) o P1). repeat split; simpl; auto; try rewrite Ht2e. rewrite sub_fit_true; auto. rewrite HP1. simpl. rewrite H1. case (eq_f (substitution f n t) (univ n B)); rewrite sub_fit_true; auto. rewrite HP4. auto. lia.
+    * simpl in C. apply f_eq_decid in Y1. destruct Y1. assert (P_proves P (lor (neg (substitution f n t)) f0) (ptree_deg P) (ptree_ord P)). repeat split; auto. assert (eq_f (lor f0 (neg (substitution f n t))) (neg (univ m f)) = false) as X0. auto.
+      assert (subst_ind_fit (lor (neg(substitution f n t)) f0) (lor_ind (0) S2) = true) as HS'. simpl. rewrite H1. auto.
+      destruct (IHP (lor (neg (substitution f n t)) f0) f m (ptree_deg P) (ptree_ord P) (contains_symm _ _ _ X0 (contains_weaken _ _ _ C)) X _ HS') as [p HC [P1 [[[HP1 HP2] HP3] HP4]]].
+      exists p; auto. exists (quantification_ad f (formula_sub_ind f0 (neg (univ m f)) (substitution (neg f) m p) S2) n t (ptree_deg P1) o P1). repeat split; simpl; auto; try rewrite Ht2e. rewrite sub_fit_true; auto. rewrite HP1. simpl. rewrite H1. case (eq_f (substitution f n t) (univ m f)); rewrite sub_fit_true; auto. rewrite HP4. auto. lia.
+    * simpl in C. assert (P_proves P (lor (neg (substitution f n t)) f0) (ptree_deg P) (ptree_ord P)). repeat split; auto. assert (eq_f (lor f0 (neg (substitution f n t))) (neg (univ m B)) = false) as X0. auto.
+      assert (subst_ind_fit (lor (neg(substitution f n t)) f0) (lor_ind (0) S2) = true) as HS'. simpl. rewrite H1. auto.
+      destruct (IHP (lor (neg (substitution f n t)) f0) B m (ptree_deg P) (ptree_ord P) (contains_symm _ _ _ X0 (contains_weaken _ _ _ C)) X _ HS') as [p HC [P1 [[[HP1 HP2] HP3] HP4]]].
+      exists p; auto. exists (quantification_ad f (formula_sub_ind f0 (neg (univ m B)) (substitution (neg B) m p) S2) n t (ptree_deg P1) o P1). repeat split; simpl; auto; try rewrite Ht2e. rewrite sub_fit_true; auto. rewrite HP1. simpl. rewrite H1. case (eq_f (substitution f n t) (univ m B)); rewrite sub_fit_true; auto. rewrite HP4. auto. lia.
+    + simpl. rewrite H1. case (eq_nat n m) eqn:Y; case (eq_f f B) eqn:Y1; simpl.
+      * case (contains_f f0 (neg (univ n f))) eqn:Y2.
+        --  apply nat_eq_decid in Y. destruct Y. apply f_eq_decid in Y1. destruct Y1. simpl. assert (P_proves P (lor (neg (substitution f n t)) f0) (ptree_deg P) (ptree_ord P)). repeat split; auto. assert (eq_f (lor f0 (neg (substitution f n t))) (neg (univ n f)) = false) as X0. auto.
+            assert (subst_ind_fit (lor (neg(substitution f n t)) f0) (lor_ind (1) S2) = true) as HS'. simpl. rewrite H1. auto.
+            destruct (IHP (lor (neg (substitution f n t)) f0) f n (ptree_deg P) (ptree_ord P) (contains_symm _ _ _ X0 (contains_weaken _ _ _ Y2)) X _ HS') as [p HC [P1 [[[HP1 HP2] HP3] HP4]]].
+            exists p; auto. exists (ord_up (ord_succ o) P1). repeat split; simpl; auto; try rewrite Ht2e. rewrite HP1. simpl. rewrite H1. assert (eq_f (substitution f n t) (univ n f) = false). admit. admit. rewrite HP4. apply ord_succ_monot. apply ord_succ_nf. apply ptree_ord_nf. auto. lia.
+        --  apply nat_eq_decid in Y. destruct Y. apply f_eq_decid in Y1. destruct Y1. exists t; auto. exists (ord_up (ord_succ (ptree_ord P)) P). rewrite not_contain_no_change_fit; auto. repeat split; simpl; auto. apply ord_succ_monot. apply ord_succ_nf. apply ptree_ord_nf. auto. lia. rewrite Ht2e. auto.
+      * simpl in C. apply nat_eq_decid in Y. destruct Y. assert (P_proves P (lor (neg (substitution f n t)) f0) (ptree_deg P) (ptree_ord P)). repeat split; auto. assert (eq_f (lor f0 (neg (substitution f n t))) (neg (univ n B)) = false) as X0. auto.
+        assert (subst_ind_fit (lor (neg(substitution f n t)) f0) (lor_ind (0) S2) = true) as HS'. simpl. rewrite H1. auto.
+        destruct (IHP (lor (neg (substitution f n t)) f0) B n (ptree_deg P) (ptree_ord P) (contains_symm _ _ _ X0 (contains_weaken _ _ _ C)) X _ HS') as [p HC [P1 [[[HP1 HP2] HP3] HP4]]].
+        exists p; auto. exists (quantification_ad f (formula_sub_ind f0 (neg (univ n B)) (substitution (neg B) n p) S2) n t (ptree_deg P1) o P1). repeat split; simpl; auto; try rewrite Ht2e. rewrite sub_fit_true; auto. rewrite HP1. simpl. rewrite H1. case (eq_f (substitution f n t) (univ n B)); rewrite sub_fit_true; auto. rewrite HP4. auto. lia.
+      * simpl in C. apply f_eq_decid in Y1. destruct Y1. assert (P_proves P (lor (neg (substitution f n t)) f0) (ptree_deg P) (ptree_ord P)). repeat split; auto. assert (eq_f (lor f0 (neg (substitution f n t))) (neg (univ m f)) = false) as X0. auto.
+        assert (subst_ind_fit (lor (neg(substitution f n t)) f0) (lor_ind (0) S2) = true) as HS'. simpl. rewrite H1. auto.
+        destruct (IHP (lor (neg (substitution f n t)) f0) f m (ptree_deg P) (ptree_ord P) (contains_symm _ _ _ X0 (contains_weaken _ _ _ C)) X _ HS') as [p HC [P1 [[[HP1 HP2] HP3] HP4]]].
+        exists p; auto. exists (quantification_ad f (formula_sub_ind f0 (neg (univ m f)) (substitution (neg f) m p) S2) n t (ptree_deg P1) o P1). repeat split; simpl; auto; try rewrite Ht2e. rewrite sub_fit_true; auto. rewrite HP1. simpl. rewrite H1. case (eq_f (substitution f n t) (univ m f)); rewrite sub_fit_true; auto. rewrite HP4. auto. lia.
+      * simpl in C. assert (P_proves P (lor (neg (substitution f n t)) f0) (ptree_deg P) (ptree_ord P)). repeat split; auto. assert (eq_f (lor f0 (neg (substitution f n t))) (neg (univ m B)) = false) as X0. auto.
+        assert (subst_ind_fit (lor (neg(substitution f n t)) f0) (lor_ind (0) S2) = true) as HS'. simpl. rewrite H1. auto.
+        destruct (IHP (lor (neg (substitution f n t)) f0) B m (ptree_deg P) (ptree_ord P) (contains_symm _ _ _ X0 (contains_weaken _ _ _ C)) X _ HS') as [p HC [P1 [[[HP1 HP2] HP3] HP4]]].
+        exists p; auto. exists (quantification_ad f (formula_sub_ind f0 (neg (univ m B)) (substitution (neg B) m p) S2) n t (ptree_deg P1) o P1). repeat split; simpl; auto; try rewrite Ht2e. rewrite sub_fit_true; auto. rewrite HP1. simpl. rewrite H1. case (eq_f (substitution f n t) (univ m B)); rewrite sub_fit_true; auto. rewrite HP4. auto. lia.
+- simpl in Ht1,Ht3,Ht4. destruct Ht1,Ht4. inversion C.
+- simpl in Ht1,Ht3,Ht4. destruct Ht1,Ht4. inversion C. simpl in Ht2. admit.
+- simpl in Ht1,Ht3,Ht4. destruct Ht2 as [[[[[[[Ht2a Ht2b] Ht2c] Ht2d] Ht2e] Ht2f] Ht2g] Ht2h]. destruct Ht1,Ht4.
+  assert (P_proves P1 (lor f f0) (ptree_deg P1) (ptree_ord P1)). repeat split; auto. assert (P_proves P2 (neg f0) (ptree_deg P2) (ptree_ord P2)). repeat split; auto. admit.
+- admit.
+- admit.
+Admitted.
+*)
+
+Lemma w_rule_invertible_a_ord : forall (alpha : ord), nf alpha -> forall (P : ptree) (A B : formula) (n d : nat),
       contains_f A (neg (univ n B)) = true -> (P_proves P A d alpha ->
             { t : term & provable (formula_sub_ind A (neg (univ n B)) (substitution (neg B) n t) (within_f A (neg (univ n B)))) d alpha & closed_t t = true}).
 Proof.
-unfold provable. induction P; intros A B m d alpha C [[[Ht1 Ht2] Ht3] Ht4].
+apply (transfinite_induction neg_invert). unfold neg_invert. unfold provable. intros alpha HA IHO P. induction P; intros A B m d C [[[Ht1 Ht2] Ht3] Ht4].
 - destruct Ht2. simpl in Ht3. apply IHP; repeat split; auto. lia.
 - destruct Ht2 as [[Ht2a Ht2b] Ht2c]. simpl in Ht1,Ht3,Ht4. destruct Ht4.
-  assert (P_proves P A (ptree_deg P) (ptree_ord P)). repeat split; auto. destruct (IHP A B m (ptree_deg P) (ptree_ord P) C X)as [p [P1 [[[HP1 HP2] HP3] HP4]]]. exists p; auto. exists (ord_up o P1). destruct HP4. repeat split; simpl; auto. lia.
+  assert (P_proves P A (ptree_deg P) (ptree_ord P)). repeat split; auto. destruct (IHO (ptree_ord P) (ptree_ord_nf _ Ht2b) Ht2a _ A B m (ptree_deg P)  C X)as [p [P1 [[[HP1 HP2] HP3] HP4]]]. exists p; auto. exists (ord_up o P1). destruct HP4. repeat split; simpl; auto. lia.
 - unfold contains_f in C. destruct A; inversion C. case (eq_f (neg A) (neg (univ m B))) eqn:X. inversion X. apply f_eq_decid in H1. rewrite H1 in *. simpl in Ht1. rewrite Ht1 in Ht2. inversion Ht2. inversion C. simpl in Ht1. rewrite Ht1 in Ht2. inversion Ht2.
 - simpl in Ht1,Ht3,Ht4. destruct Ht2 as [[[Ht2a Ht2b] Ht2c] Ht2d]. destruct Ht1,Ht4.
-  assert (P_proves P (lor f f0) (ptree_deg P) (ptree_ord P)). repeat split; auto. assert (eq_f (lor f0 f) (neg (univ m B)) = false) as X0. auto.
-  destruct (IHP (lor f f0) B m (ptree_deg P) (ptree_ord P) (contains_symm _ _ _ X0 C) X)as [p [P1 [[[HP1 HP2] HP3] HP4]]]. exists p; auto. exists (exchange_ab (formula_sub_ind f (neg (univ m B)) (substitution (neg B) m p) (within_f f (neg (univ m B)))) (formula_sub_ind f0 (neg (univ m B)) (substitution (neg B) m p) (within_f f0 (neg (univ m B)))) (ptree_deg P1) o P1). destruct HP4. repeat split; simpl; auto.
+  assert (P_proves P (lor f f0) (ptree_deg P) (ptree_ord P)). repeat split; auto. assert (eq_f (lor f0 f) (neg (univ m B)) = false) as X0. auto. rewrite Ht2d in IHP.
+  destruct (IHP (lor f f0) B m (ptree_deg P) (contains_symm _ _ _ X0 C) X)as [p [P1 [[[HP1 HP2] HP3] HP4]]]. exists p; auto. exists (exchange_ab (formula_sub_ind f (neg (univ m B)) (substitution (neg B) m p) (within_f f (neg (univ m B)))) (formula_sub_ind f0 (neg (univ m B)) (substitution (neg B) m p) (within_f f0 (neg (univ m B)))) (ptree_deg P1) o P1). destruct HP4. repeat split; simpl; auto.
   rewrite within_fits. rewrite within_fits. simpl. rewrite sub_fit_true. rewrite sub_fit_true. auto. apply within_fits. apply within_fits. rewrite <- formula_sub_ind_lor. auto. rewrite within_fits. apply within_fits. lia.
 - simpl in Ht1,Ht3,Ht4. destruct Ht2 as [[[Ht2a Ht2b] Ht2c] Ht2d]. destruct Ht1,Ht4.
-  assert (P_proves P (lor (lor f f0) f1) (ptree_deg P) (ptree_ord P)). repeat split; auto. assert (eq_f (lor (lor f f1) f0) (neg (univ m B)) = false) as X0. auto. assert (eq_f (lor f0 f) (neg (univ m B)) = false) as X1. auto.
-  destruct (IHP (lor (lor f f0) f1) B m (ptree_deg P) (ptree_ord P) (contains_swap_end _ _ _ _ X0 X1 C) X)as [p [P1 [[[HP1 HP2] HP3] HP4]]]. exists p; auto. exists (exchange_cab (formula_sub_ind f (neg (univ m B)) (substitution (neg B) m p) (within_f f (neg (univ m B)))) (formula_sub_ind f0 (neg (univ m B)) (substitution (neg B) m p) (within_f f0 (neg (univ m B)))) (formula_sub_ind f1 (neg (univ m B)) (substitution (neg B) m p) (within_f f1 (neg (univ m B)))) (ptree_deg P1) o P1). destruct HP4. repeat split; simpl; auto.
+  assert (P_proves P (lor (lor f f0) f1) (ptree_deg P) (ptree_ord P)). repeat split; auto. assert (eq_f (lor (lor f f1) f0) (neg (univ m B)) = false) as X0. auto. assert (eq_f (lor f0 f) (neg (univ m B)) = false) as X1. auto. rewrite Ht2d in IHP.
+  destruct (IHP (lor (lor f f0) f1) B m (ptree_deg P) (contains_swap_end _ _ _ _ X0 X1 C) X) as [p [P1 [[[HP1 HP2] HP3] HP4]]]. exists p; auto. exists (exchange_cab (formula_sub_ind f (neg (univ m B)) (substitution (neg B) m p) (within_f f (neg (univ m B)))) (formula_sub_ind f0 (neg (univ m B)) (substitution (neg B) m p) (within_f f0 (neg (univ m B)))) (formula_sub_ind f1 (neg (univ m B)) (substitution (neg B) m p) (within_f f1 (neg (univ m B)))) (ptree_deg P1) o P1). destruct HP4. repeat split; simpl; auto.
   repeat rewrite within_fits. simpl. repeat rewrite sub_fit_true. auto. apply within_fits. apply within_fits. apply within_fits. repeat rewrite <- formula_sub_ind_lor. auto. unfold subst_ind_fit. fold subst_ind_fit. repeat rewrite within_fits. auto. repeat rewrite within_fits. auto. lia.
 - simpl in Ht1,Ht3,Ht4. destruct Ht2 as [[[Ht2a Ht2b] Ht2c] Ht2d]. destruct Ht1,Ht4.
-  assert (P_proves P (lor (lor f f0) f1) (ptree_deg P) (ptree_ord P)). repeat split; auto. assert (eq_f (lor (lor f0 f) f1) (neg (univ m B)) = false) as X0. auto. assert (eq_f (lor f0 f) (neg (univ m B)) = false) as X1. auto.
-  destruct (IHP (lor (lor f f0) f1) B m (ptree_deg P) (ptree_ord P) (contains_swap_start _ _ _ _ X0 X1 C) X)as [p [P1 [[[HP1 HP2] HP3] HP4]]]. exists p; auto. exists (exchange_abd (formula_sub_ind f (neg (univ m B)) (substitution (neg B) m p) (within_f f (neg (univ m B)))) (formula_sub_ind f0 (neg (univ m B)) (substitution (neg B) m p) (within_f f0 (neg (univ m B)))) (formula_sub_ind f1 (neg (univ m B)) (substitution (neg B) m p) (within_f f1 (neg (univ m B)))) (ptree_deg P1) o P1). destruct HP4. repeat split; simpl; auto.
+  assert (P_proves P (lor (lor f f0) f1) (ptree_deg P) (ptree_ord P)). repeat split; auto. assert (eq_f (lor (lor f0 f) f1) (neg (univ m B)) = false) as X0. auto. assert (eq_f (lor f0 f) (neg (univ m B)) = false) as X1. auto. rewrite Ht2d in IHP.
+  destruct (IHP (lor (lor f f0) f1) B m (ptree_deg P) (contains_swap_start _ _ _ _ X0 X1 C) X) as [p [P1 [[[HP1 HP2] HP3] HP4]]]. exists p; auto. exists (exchange_abd (formula_sub_ind f (neg (univ m B)) (substitution (neg B) m p) (within_f f (neg (univ m B)))) (formula_sub_ind f0 (neg (univ m B)) (substitution (neg B) m p) (within_f f0 (neg (univ m B)))) (formula_sub_ind f1 (neg (univ m B)) (substitution (neg B) m p) (within_f f1 (neg (univ m B)))) (ptree_deg P1) o P1). destruct HP4. repeat split; simpl; auto.
   repeat rewrite within_fits. simpl. repeat rewrite sub_fit_true. auto. apply within_fits. apply within_fits. apply within_fits. repeat rewrite <- formula_sub_ind_lor. auto. unfold subst_ind_fit. fold subst_ind_fit. repeat rewrite within_fits. auto. repeat rewrite within_fits. auto. lia.
 - simpl in Ht1,Ht3,Ht4. destruct Ht2 as [[[Ht2a Ht2b] Ht2c] Ht2d]. destruct Ht1,Ht4.
-  assert (P_proves P (lor (lor (lor f f0) f1) f2) (ptree_deg P) (ptree_ord P)). repeat split; auto. assert (eq_f (lor (lor (lor f f1) f0) f2) (neg (univ m B)) = false) as X0. auto. assert (eq_f (lor (lor f f1) f0) (neg (univ m B)) = false) as X1. auto. assert (eq_f (lor f f1) (neg (univ m B)) = false) as X2. auto.
-  destruct (IHP (lor (lor (lor f f0) f1) f2) B m (ptree_deg P) (ptree_ord P) (contains_swap_mid _ _ _ _ _ X0 X1 X2 C) X)as [p [P1 [[[HP1 HP2] HP3] HP4]]]. exists p; auto. exists (exchange_cabd (formula_sub_ind f (neg (univ m B)) (substitution (neg B) m p) (within_f f (neg (univ m B)))) (formula_sub_ind f0 (neg (univ m B)) (substitution (neg B) m p) (within_f f0 (neg (univ m B)))) (formula_sub_ind f1 (neg (univ m B)) (substitution (neg B) m p) (within_f f1 (neg (univ m B)))) (formula_sub_ind f2 (neg (univ m B)) (substitution (neg B) m p) (within_f f2 (neg (univ m B)))) (ptree_deg P1) o P1). destruct HP4. repeat split; simpl; auto.
+  assert (P_proves P (lor (lor (lor f f0) f1) f2) (ptree_deg P) (ptree_ord P)). repeat split; auto. assert (eq_f (lor (lor (lor f f1) f0) f2) (neg (univ m B)) = false) as X0. auto. assert (eq_f (lor (lor f f1) f0) (neg (univ m B)) = false) as X1. auto. assert (eq_f (lor f f1) (neg (univ m B)) = false) as X2. auto. rewrite Ht2d in IHP.
+  destruct (IHP (lor (lor (lor f f0) f1) f2) B m (ptree_deg P) (contains_swap_mid _ _ _ _ _ X0 X1 X2 C) X) as [p [P1 [[[HP1 HP2] HP3] HP4]]]. exists p; auto. exists (exchange_cabd (formula_sub_ind f (neg (univ m B)) (substitution (neg B) m p) (within_f f (neg (univ m B)))) (formula_sub_ind f0 (neg (univ m B)) (substitution (neg B) m p) (within_f f0 (neg (univ m B)))) (formula_sub_ind f1 (neg (univ m B)) (substitution (neg B) m p) (within_f f1 (neg (univ m B)))) (formula_sub_ind f2 (neg (univ m B)) (substitution (neg B) m p) (within_f f2 (neg (univ m B)))) (ptree_deg P1) o P1). destruct HP4. repeat split; simpl; auto.
   repeat rewrite within_fits. simpl. repeat rewrite sub_fit_true. auto. apply within_fits. apply within_fits. apply within_fits. apply within_fits. repeat rewrite <- formula_sub_ind_lor. auto. unfold subst_ind_fit. fold subst_ind_fit. repeat rewrite within_fits. auto. unfold subst_ind_fit. fold subst_ind_fit. repeat rewrite within_fits. auto. repeat rewrite within_fits. auto. lia.
 - simpl in Ht1,Ht3,Ht4. destruct Ht2 as [[[Ht2a Ht2b] Ht2c] Ht2d]. destruct Ht1,Ht4.
-  assert (P_proves P (lor f f) (ptree_deg P) (ptree_ord P)). repeat split; auto.
-  destruct (IHP (lor f f) B m (ptree_deg P) (ptree_ord P) (contains_weaken  _ f _ C) X) as [p [P1 [[[HP1 HP2] HP3] HP4]]]. exists p; auto. exists (contraction_a (formula_sub_ind f (neg (univ m B)) (substitution (neg B) m p) (within_f f (neg (univ m B)))) (ptree_deg P1) o P1). destruct HP4. repeat split; simpl; auto.
+  assert (P_proves P (lor f f) (ptree_deg P) (ptree_ord P)). repeat split; auto. rewrite Ht2d in IHP.
+  destruct (IHP (lor f f) B m (ptree_deg P) (contains_weaken  _ f _ C) X) as [p [P1 [[[HP1 HP2] HP3] HP4]]]. exists p; auto. exists (contraction_a (formula_sub_ind f (neg (univ m B)) (substitution (neg B) m p) (within_f f (neg (univ m B)))) (ptree_deg P1) o P1). destruct HP4. repeat split; simpl; auto.
   rewrite <- formula_sub_ind_lor. auto. rewrite within_fits. auto. lia.
 - simpl in Ht1,Ht3,Ht4. destruct Ht2 as [[[Ht2a Ht2b] Ht2c] Ht2d]. destruct Ht1,Ht4.
-  assert (P_proves P (lor (lor f f) f0) (ptree_deg P) (ptree_ord P)). repeat split; auto. assert (eq_f (lor (lor f f0) f) (neg (univ m B)) = false) as X0. auto. assert (eq_f (lor f f0) (neg (univ m B)) = false) as X1. auto.
-  destruct (IHP (lor (lor f f) f0) B m (ptree_deg P) (ptree_ord P) (contains_swap_end _ _ _ _ X0 X1 (contains_weaken  _ f _ C)) X) as [p [P1 [[[HP1 HP2] HP3] HP4]]]. exists p; auto. exists (contraction_ad (formula_sub_ind f (neg (univ m B)) (substitution (neg B) m p) (within_f f (neg (univ m B)))) (formula_sub_ind f0 (neg (univ m B)) (substitution (neg B) m p) (within_f f0 (neg (univ m B)))) (ptree_deg P1) o P1). destruct HP4. repeat split; simpl; auto.
+  assert (P_proves P (lor (lor f f) f0) (ptree_deg P) (ptree_ord P)). repeat split; auto. assert (eq_f (lor (lor f f0) f) (neg (univ m B)) = false) as X0. auto. assert (eq_f (lor f f0) (neg (univ m B)) = false) as X1. auto. rewrite Ht2d in IHP.
+  destruct (IHP (lor (lor f f) f0) B m (ptree_deg P) (contains_swap_end _ _ _ _ X0 X1 (contains_weaken  _ f _ C)) X) as [p [P1 [[[HP1 HP2] HP3] HP4]]]. exists p; auto. exists (contraction_ad (formula_sub_ind f (neg (univ m B)) (substitution (neg B) m p) (within_f f (neg (univ m B)))) (formula_sub_ind f0 (neg (univ m B)) (substitution (neg B) m p) (within_f f0 (neg (univ m B)))) (ptree_deg P1) o P1). destruct HP4. repeat split; simpl; auto.
   rewrite <- formula_sub_ind_lor. auto. repeat rewrite within_fits. auto. repeat rewrite <- formula_sub_ind_lor. auto. simpl. repeat rewrite within_fits. auto. repeat rewrite within_fits. auto. lia.
 - simpl in Ht1,Ht3,Ht4. destruct Ht2 as [[[[Ht2a Ht2b] Ht2c] Ht2d] Ht2e]. destruct Ht1. simpl in C. apply or_bool_prop in C. case (contains_f f0 (neg (univ m B))) eqn:Y.
-  + assert (P_proves P f0 (ptree_deg P) (ptree_ord P)). repeat split; auto.
-  destruct (IHP f0 B m (ptree_deg P) (ptree_ord P) Y X) as [p [P1 [[[HP1 HP2] HP3] HP4]]]. exists p; auto. exists (weakening_ad (formula_sub_ind f (neg (univ m B)) (substitution (neg B) m p) (within_f f (neg (univ m B)))) (formula_sub_ind f0 (neg (univ m B)) (substitution (neg B) m p) (within_f f0 (neg (univ m B)))) (ptree_deg P1) o P1). destruct HP4. repeat split; simpl; auto.
-  rewrite <- formula_sub_ind_lor. auto. repeat rewrite within_fits. auto. apply formula_sub_ind_closed; auto. intros. apply closed_univ_sub; auto. lia.
+  + assert (P_proves P f0 (ptree_deg P) (ptree_ord P)). repeat split; auto. rewrite Ht2e in Ht4. rewrite <- Ht4 in IHO.
+  destruct (IHO (ptree_ord P) (ptree_ord_nf _ Ht2c) (ord_succ_monot _) _ f0 B m (ptree_deg P) Y X) as [p [P1 [[[HP1 HP2] HP3] HP4]]]. exists p; auto. exists (weakening_ad (formula_sub_ind f (neg (univ m B)) (substitution (neg B) m p) (within_f f (neg (univ m B)))) (formula_sub_ind f0 (neg (univ m B)) (substitution (neg B) m p) (within_f f0 (neg (univ m B)))) (ptree_deg P1) o P1). destruct HP4. repeat split; simpl; auto.
+  rewrite <- formula_sub_ind_lor. auto. repeat rewrite within_fits. auto. apply formula_sub_ind_closed; auto. intros. apply closed_univ_sub; auto. lia. rewrite Ht2e. auto.
   + exists (represent 0); auto. exists (weakening_ad (formula_sub_ind f (neg (univ m B)) (substitution (neg B) m (represent 0)) (within_f f (neg (univ m B)))) f0 n o P). repeat split; auto.
     simpl. rewrite (not_contain_non_tatget f0); auto. rewrite non_target_fit. repeat rewrite within_fits. simpl. rewrite non_target_sub'. rewrite sub_fit_true. auto. apply within_fits.  inversion C; inversion H. rewrite H. pose (contains_closed _ _ Ht2b H). apply formula_sub_ind_closed; auto. intros. apply closed_univ_sub; auto.
 - admit.
 - admit.
 - simpl in Ht1,Ht3,Ht4. destruct Ht2 as [[[Ht2a Ht2b] Ht2c] Ht2d]. destruct Ht1,Ht4. simpl in C. inversion C.
 - simpl in Ht1,Ht3,Ht4. destruct Ht2 as [[[Ht2a Ht2b] Ht2c] Ht2d]. destruct Ht1,Ht4. simpl in C.  
-  assert (P_proves P (lor f f0) (ptree_deg P) (ptree_ord P)). repeat split; auto. assert (eq_f (lor f0 f) (neg (univ m B)) = false) as X0. auto.
-  destruct (IHP (lor f f0) B m (ptree_deg P) (ptree_ord P) (contains_symm _ _ _ X0 (contains_weaken _ _ _ C)) X) as [p [P1 [[[HP1 HP2] HP3] HP4]]]. case (contains_f f (neg (univ m B))) eqn:Y.
+  assert (P_proves P (lor f f0) (ptree_deg P) (ptree_ord P)). repeat split; auto. assert (eq_f (lor f0 f) (neg (univ m B)) = false) as X0. auto. rewrite Ht2d in IHO.
+  destruct (IHO (ptree_ord P) (ptree_ord_nf _ Ht2b) (ord_succ_monot _) P (lor f f0) B m (ptree_deg P) (contains_symm _ _ _ X0 (contains_weaken _ _ _ C)) X) as [p [P1 [[[HP1 HP2] HP3] HP4]]]. case (contains_f f (neg (univ m B))) eqn:Y.
   + exists p; auto. exists (negation_ad f (formula_sub_ind f0 (neg (univ m B)) (substitution (neg B) m p) (within_f f0 (neg (univ m B)))) (ptree_deg P1) o P1). destruct HP4. repeat split; simpl; auto.
-    rewrite within_fits. rewrite sub_fit_true; auto. apply within_fits. auto. repeat rewrite within_fits. auto. admit. lia.
+    rewrite within_fits. rewrite sub_fit_true; auto. apply within_fits. rewrite HP1. admit. lia.
   + exists p; auto. exists (negation_ad f (formula_sub_ind f0 (neg (univ m B)) (substitution (neg B) m p) (within_f f0 (neg (univ m B)))) (ptree_deg P1) o P1). destruct HP4. repeat split; simpl; auto.
     rewrite within_fits. rewrite sub_fit_true; auto. apply within_fits. simpl in HP1. repeat rewrite within_fits in HP1. simpl in HP1. rewrite not_contain_non_tatget in HP1; auto. rewrite <- sub_fit_true in HP1. rewrite <- sub_fit_true in HP1. rewrite non_target_sub in HP1. auto. apply within_fits. apply non_target_fit. lia.
 
@@ -197,15 +511,11 @@ unfold provable. induction P; intros A B m d alpha C [[[Ht1 Ht2] Ht3] Ht4].
 - simpl in Ht1,Ht3,Ht4. destruct Ht1,Ht4. inversion C.
 - simpl in Ht1,Ht3,Ht4. destruct Ht1,Ht4. inversion C. simpl in Ht2. admit.
 - simpl in Ht1,Ht3,Ht4. destruct Ht2 as [[[[[[[Ht2a Ht2b] Ht2c] Ht2d] Ht2e] Ht2f] Ht2g] Ht2h]. destruct Ht1,Ht4.
-  assert (P_proves P1 (lor f f0) (ptree_deg P1) (ptree_ord P1)). repeat split; auto. assert (P_proves P2 (neg f0) (ptree_deg P2) (ptree_ord P2)). repeat split; auto.
-  
-  assert (eq_f (lor (lor f f0) f) (neg (univ m B)) = false) as X0. auto. assert (eq_f (lor f f0) (neg (univ m B)) = false) as X1. auto.
-  destruct (IHP (lor (lor f f) f0) B m (ptree_deg P) (ptree_ord P) (contains_swap_end _ _ _ _ X0 X1 (contains_weaken  _ f _ C)) X) as [p [P1 [[[HP1 HP2] HP3] HP4]]]. exists p; auto. exists (contraction_ad (formula_sub_ind f (neg (univ m B)) (substitution (neg B) m p) (within_f f (neg (univ m B)))) (formula_sub_ind f0 (neg (univ m B)) (substitution (neg B) m p) (within_f f0 (neg (univ m B)))) (ptree_deg P1) o P1). destruct HP4. repeat split; simpl; auto.
-  rewrite <- formula_sub_ind_lor. auto. repeat rewrite within_fits. auto. repeat rewrite <- formula_sub_ind_lor. auto. simpl. repeat rewrite within_fits. auto. repeat rewrite within_fits. auto. lia.
-
+  assert (P_proves P1 (lor f f0) (ptree_deg P1) (ptree_ord P1)). repeat split; auto. assert (P_proves P2 (neg f0) (ptree_deg P2) (ptree_ord P2)). repeat split; auto. admit.
 - admit.
 - admit.
 Admitted.
+
 
 
 Lemma w_rule_invertible_a :
